要证：

对于任意 $x$，$\sin{{3}{x}} = 3 * \sin{x} - 4 * \sin{x}^{3}$

证明：

我们有: $\sin{{3}{x}} = \sin{({2}{x} + x)} = \sin{{2}{x}} * \cos{x} + \cos{{2}{x}} * \sin{x} $,

我们知道 $\sin{{2}{x}} * \cos{x} = (2 * \sin{x} * \cos{x}) * \cos{x} = 2 * \sin{x} * \cos{x} ^ {2} = 2 * \sin{x} * (1 - \sin{x} ^ {2}) = 2 * \sin{x} - 2 * \sin{x} ^ {3}$,

我们知道 $\cos{{2}{x}} * \sin{x} = (1 - 2 * \sin{x} ^ {2}) * \sin{x} = \sin{x} - 2 * \sin{x} ^ {3}$,

因此 $\sin{{3}{x}} = \sin{{2}{x}} * \cos{x} + \cos{{2}{x}} * \sin{x} = (2 * \sin{x} - 2 * \sin{x} ^ {3}) + (\sin{x} - 2 * \sin{x} ^ {3}) = 3 * \sin{x} - 4 * \sin{x}^{3}$,

综上可知，原命题得证。