要证：

对于任意 $x$，$\frac{\sin{({5}{x})}}{\sin{({2}{x})}} + \frac{\sin{({2}{x})}}{\sin{x}} = \frac{\sin{({3}{x})}^{2}}{\sin{({2}{x})}*\sin{x}}$

证明：

我们有: $\sin{({5}{x})} * \sin{x} = \sin{(({3}{x}) + ({2}{x}))} * \sin{(({3}{x}) - ({2}{x}))} = (\sin{({3}{x})}*\cos{({2}{x})} + \cos{({3}{x})}*\sin{({2}{x})}) *(\sin{({3}{x})}*\cos{({2}{x})} - \cos{({3}{x})}*\sin{({2}{x})}) = \sin{({3}{x})}^{2} * \cos{({2}{x})}^{2} - \sin{({2}{x})}^{2} * \cos{({3}{x})}^{2} =  \sin{({3}{x})}^{2} * (1 - \sin{({2}{x})}^{2}) - \sin{({2}{x})}^{2} * (1 - \sin{({3}{x})}^{2}) = \sin{({3}{x})}^{2} - \sin{({2}{x})}^{2}$,

因此，$\frac{\sin{({5}{x})}}{\sin{({2}{x})}} + \frac{\sin{({2}{x})}}{\sin{x}} = \frac{\sin{({5}{x})} * \sin{x} + \sin{({2}{x})} ^ {2}}{\sin{({2}{x})}*\sin{x}} = \frac{(\sin{({3}{x})}^{2} - \sin{({2}{x})}^{2}) + (\sin{({2}{x})}) ^ {2}}{\sin{({2}{x})}*\sin{x}} = \frac{\sin{({3}{x})}^{2}}{\sin{({2}{x})}*\sin{x}}$,

综上可知，原命题得证。
