要证：

对于任意 $x$，$\sin{(x - \frac{2*\pi}{3})} + \sin{x} + \sin{(x + \frac{2*\pi}{3})} = 0$

证明：

我们有: $\sin{(x - \frac{2*\pi}{3})} = \sin{x}*\cos{\frac{2*\pi}{3}} - \cos{x}*\sin{\frac{2*\pi}{3}} = (-\frac{1}{2})*\sin{x} - \frac{\sqrt{3}}{2}*\cos{x}$,

同样地，$\sin{(x + \frac{2*\pi}{3})} = \sin{x}*\cos{\frac{2*\pi}{3}} + \cos{x}*\sin{\frac{2*\pi}{3}} = (-\frac{1}{2})*\sin{x} + \frac{\sqrt{3}}{2}*\cos{x}$,

因此，$\sin{(x - \frac{2*\pi}{3})} + \sin{x} + \sin{(x + \frac{2*\pi}{3})} = ((-\frac{1}{2})*\sin{x} - \frac{\sqrt{3}}{2}*\cos{x}) + \sin{x} + ((-\frac{1}{2})*\sin{x} + \frac{\sqrt{3}}{2}*\cos{x}) = (1 - \frac{1}{2} - \frac{1}{2}) * \sin{x} + (\frac{\sqrt{3}}{2} - \frac{\sqrt{3}}{2}) * \cos{x} = 0$,

综上可知，原命题得证。