要证：

对于任意 $a$，$ \cos{\frac{a}{2^{3}}} * \cos{\frac{a}{2^{2}}} * \cos{\frac{a}{2}} = \frac{1}{2^{3}}*\frac{\sin{a}}{\sin{\frac{a}{2^{3}}}}$

证明：

我们有: $\sin{\frac{a}{2^{3}}} * \cos{\frac{a}{2^{3}}} = \frac{\sin{2*\frac{a}{2^{3}}}}{2} = \frac{\sin{\frac{a}{2^{2}}}}{2}$,

我们有: $\sin{\frac{a}{2^{2}}} * \cos{\frac{a}{2^{2}}} = \frac{\sin{2*\frac{a}{2^{2}}}}{2} = \frac{\sin{\frac{a}{2}}}{2}$,

我们有: $\sin{\frac{a}{2}} * \cos{\frac{a}{2}} = \frac{\sin{2*\frac{a}{2}}}{2} = \frac{\sin{a}}{2}$,

因此，$\sin{\frac{a}{2^{3}}} * \cos{\frac{a}{2^{3}}} * \cos{\frac{a}{2^{2}}} * \cos{\frac{a}{2}} = \frac{\sin{\frac{a}{2^{2}}}}{2} * \cos{\frac{a}{2^{2}}} * \cos{\frac{a}{2}} = \frac{1}{2} * (\sin{\frac{a}{2^{2}}} * \cos{\frac{a}{2^{2}}}) * \cos{\frac{a}{2}} = \frac{1}{2} * (\frac{\sin{\frac{a}{2}}}{2}) * \cos{\frac{a}{2}} = \frac{1}{2^{2}} * (\sin{\frac{a}{2}} * \cos{\frac{a}{2}}) = \frac{1}{2^{2}} * (\frac{\sin{a}}{2}) = \frac{\sin{a}}{2^{3}} $,

由___hyp6式变形得：$ \cos{\frac{a}{2^{3}}} * \cos{\frac{a}{2^{2}}} * \cos{\frac{a}{2}} = \frac{1}{2^{3}}*\frac{\sin{a}}{\sin{\frac{a}{2^{3}}}} $,


综上可知，原命题得证。