已知：
$f(x) := (x + 1) * (x + 2) ^ {2} * (x + 3) ^ {3}$

Goal:
$$f'(x) = (\frac{1}{x + 1} + \frac{2}{x + 2} + \frac{3}{x + 3}) * (x + 1) * (x + 2) ^ {2} * (x + 3) ^ {3}$$

证：

易知：
$$\ln{(f(x))} = \ln{(x + 1)} + 2 * \ln{(x + 2)} + 3 * \ln{(x + 3)}$$

两边对x求导：
$$\frac{f'(x)}{f(x)} = \frac{1}{x + 1} + \frac{2}{x + 2} + \frac{3}{x + 3}$$

由___hyp2式等价变形得：
$$f'(x) = (\frac{1}{x + 1} + \frac{2}{x + 2} + \frac{3}{x + 3}) * f(x)$$

易知：
$$f'(x) = (\frac{1}{x + 1} + \frac{2}{x + 2} + \frac{3}{x + 3}) * (x + 1) * (x + 2) ^ {2} * (x + 3) ^ {3}$$

综上可知，原命题得证。
