要证：
$$\forall a b c d$$
$${(a^{2} + b^{2})}{(c^{2} + d^{2})} \ge ({a}{c} + {b}{d})^{2}$$

证明：

易知：
$$ {(a^{2} + b^{2})}{(c^{2} + d^{2})} = {a^{2}}{c^{2}} + {a^{2}}{d^{2}} + {b^{2}}{c^{2}} + {b^{2}}{d^{2}} = ({a^{2}}{c^{2}} + 2*({a}{c})*({b}{d}) + {b^{2}}{d^{2}}) + ({a^{2}}{d^{2}} - 2*({a}{d})*({b}{c}) + {b^{2}}{c^{2}}) = ({a}{c} + {b}{d})^{2} + ({a}{d} - {b}{c})^{2} $$
,

因此，
$${(a^{2} + b^{2})}{(c^{2} + d^{2})} = ({a}{c} + {b}{d})^{2} + ({a}{d} - {b}{c})^{2} \ge ({a}{c} + {b}{d})^{2}$$
,

综上可知，原命题得证。