要证：
对于任意 $x$，$\ln{(x * \sqrt{\frac{e^{3} * x}{1 - x}})} = \frac{3}{2} + \frac{3}{2} * \ln{(x)} - \frac{1}{2} * \ln{(1 - x)}$

证：

易知：
$\ln{(x * \sqrt{\frac{e^{3} * x}{1 - x}})} = \ln{(x)} + \ln{(\sqrt{\frac{e^{3} * x}{1 - x}})} = \ln{(x)} + \frac{1}{2} * \ln{(\frac{e^{3} * x}{1 - x})} = \ln{(x)} + \frac{1}{2} * (\ln{(e^{3} * x)} - \ln{(1 - x)}) = \ln{(x)} + \frac{1}{2} * (\ln{(e^{3})} + \ln{(x)} - \ln{(1 - x)}) = \frac{\ln{(e^{3})}}{2} + \frac{3}{2} * \ln{(x)} - \frac{1}{2} * \ln{(1 - x)} = \frac{3}{2} + \frac{3}{2} * \ln{(x)} - \frac{1}{2} * \ln{(1 - x)} $,


综上可知，原命题得证。